src/cbor/CBOR.Spec.Raw.Map.fst
@@ -484,7 +484,7 @@ let list_memP_map_forall
 = Classical.forall_intro (fun y -> List.Tot.memP_map_elim f y l);
   Classical.forall_intro (fun x -> List.Tot.memP_map_intro f x l)
 
-#push-options "--z3rlimit 32"
+#push-options "--z3rlimit 64"
 
 #restart-solver
 let rec map_sort_correct
